fix main proof

src/Find_tree_stack.thy
@@ -7,23 +7,28 @@ begin
    guaranteed to be a leaf; also include the key we are looking
    for; also include bounds on the keys that we may find
 *)
-datatype fts_state = Fts_state "key * Tree * context_t"
 
-definition dest_fts_state :: "fts_state => (key * Tree * context_t)" where
-"dest_fts_state fts == (case fts of Fts_state (k,t,c) => (k,t,c))"
+(*begin f focus definition*)
+type_synonym f_focus_t = "key * Tree"
+(*end f focus definition*)
 
-definition tree_to_fts :: "key => Tree => fts_state" where
+type_synonym f_tree_stack = "f_focus_t tree_stack"
+
+definition dest_f_tree_stack :: "f_tree_stack => (key * Tree * context_t)" where
+"dest_f_tree_stack fts = (case fts of (Tree_stack (Focus (k,t), ctx)) => (k,t,ctx))"
+
+definition tree_to_fts :: "key => Tree => f_tree_stack" where
 "tree_to_fts k t == (
-Fts_state (k,t,Nil))"
+Tree_stack (Focus (k,t),Nil))"
 
 (* tr: link between focus and context?*)
 definition wellformed_fts_focus :: "ms_t => Tree => bool" where
 "wellformed_fts_focus ms t == (
 wellformed_tree ms t)"
 
-definition wellformed_fts_1 :: "fts_state => bool" where
+definition wellformed_fts_1 :: "f_tree_stack => bool" where
 "wellformed_fts_1 fts == (
-let (k,t,ctx) = dest_fts_state fts in
+let (k,t,ctx) = dest_f_tree_stack fts in
 (case ctx of
 Nil => True
 | x#xs =>
@@ -34,18 +39,18 @@ Nil => True
  (check_keys l [k] u)
 ))"
 
-definition wellformed_fts :: "fts_state => bool" where
+definition wellformed_fts :: "f_tree_stack => bool" where
 "wellformed_fts fts == (
-let (k,t,ctx) = dest_fts_state fts in
+let (k,t,ctx) = dest_f_tree_stack fts in
 let ms = if (ctx = Nil) then (Some Small_root_node_or_leaf) else None in
 wellformed_fts_focus ms t
 & wellformed_context ctx
 & wellformed_fts_1 fts)"
 
 (*tr: stops when gets to leaf; no "errors"*)
-definition step_fts :: "fts_state => fts_state option" where
+definition step_fts :: "f_tree_stack => f_tree_stack option" where
 "step_fts fts == (
-let (k,t,ctx) = dest_fts_state fts in
+let (k,t,ctx) = dest_f_tree_stack fts in
 let (lb,rb) =
  case ctx of Nil => (None,None)
  | (lb,_,rb)#_ => (lb, rb) 
@@ -56,7 +61,7 @@ Leaf _ => None
  let i = search_key_to_index ks k in
  let (l,u) = get_lower_upper_keys_for_node_t ks lb i rb in
  let ctx2 = (l,((ks,rs),i),u)#ctx in
- Some(Fts_state(k,(rs!i),ctx2))
+ Some(Tree_stack(Focus(k,(rs!i)),ctx2))
 ))"
 
 declare [[code abort: key_lt]]
